Phi_Semantics/PhiSem_CF_Routine.thy
@@ -17,12 +17,12 @@ lemma "__routine__":
 \<Longrightarrow> \<phi>_Have_Types Y TY_RETs
 \<Longrightarrow> \<r>Success
 \<Longrightarrow> (\<And>(vs:: 'a::FIX_ARITY_VALs \<phi>arg <named> 'names) label_ret.
-      return_\<phi>app\<^bold>: HIDDEN_PREM(
+      return_\<phi>app\<^bold>: TECHNICAL(
           \<forall>ret :: 'b :: FIX_ARITY_VALs \<phi>arg.
-            \<p>\<r>\<o>\<c> (op_break label_ret ret :: 'b proc) \<lbrace> Y ret\<heavy_comma> Brk_Frame label_ret \<longmapsto> 0 \<rbrace>
+            \<p>\<r>\<o>\<c> (op_break label_ret ret :: 'b proc) \<lbrace> Y ret\<heavy_comma> TECHNICAL Brk_Frame label_ret \<longmapsto> 0 \<rbrace>
             \<t>\<h>\<r>\<o>\<w>\<s> (\<lambda>_. Brking_Frame label_ret Y))
-      \<Longrightarrow> \<p>\<r>\<o>\<c> F label_ret (case_named (\<lambda>x. x) vs) \<lbrace> X (case_named id vs)\<heavy_comma> Brk_Frame label_ret
-                                          \<longmapsto> \<lambda>ret. Y ret\<heavy_comma> Brk_Frame label_ret
+      \<Longrightarrow> \<p>\<r>\<o>\<c> F label_ret (case_named (\<lambda>x. x) vs) \<lbrace> X (case_named id vs)\<heavy_comma> TECHNICAL Brk_Frame label_ret
+                                          \<longmapsto> \<lambda>ret. Y ret\<heavy_comma> TECHNICAL Brk_Frame label_ret
                                             \<rbrace> \<t>\<h>\<r>\<o>\<w>\<s> (\<lambda>e. \<^bold>b\<^bold>r\<^bold>e\<^bold>a\<^bold>k label_ret \<^bold>w\<^bold>i\<^bold>t\<^bold>h Y \<^bold>o\<^bold>r E e))
 \<Longrightarrow> \<p>\<r>\<o>\<c> op_routine TY_ARGs TY_RETs F vs \<lbrace> X vs \<longmapsto> Y \<rbrace> \<t>\<h>\<r>\<o>\<w>\<s> E\<close>
   unfolding op_routine_def
@@ -30,7 +30,7 @@ lemma "__routine__":
     "__routine_basic__"[where TY_ARGs=TY_ARGs and TY_RETs=TY_RETs and X=X and Y=Y and vs=vs and 'names='names, simplified]
     \<medium_left_bracket> for vs
       brk_scope \<medium_left_bracket> for label_ret
-        F[where vs=\<open>tag vs\<close>, unfolded HIDDEN_PREM_def, simplified]
+        F[where vs=\<open>tag vs\<close>, unfolded Technical_def[where 'a=\<open>bool\<close>], simplified]
         "_op_break_rule_"
       \<medium_right_bracket>. ;;
     \<medium_right_bracket>. ;;
