Phi_Semantics/PhiSem_Play_Ground.thy
@@ -100,17 +100,20 @@ proc
   output \<open>\<v>\<a>\<l> a + b + c \<Ztypecolon> \<nat>\<^sup>r('b)\<close>
   \<medium_left_bracket> ;; \<open>$a + $b + $c\<close> \<medium_right_bracket>. .
 
+declare [[\<phi>hide_techinicals=true]]
+
+thm while_\<phi>app
 
 proc
   input \<open>\<v>\<a>\<l> x \<Ztypecolon> \<nat>\<close>
   premises \<open>x < 10\<close>
   output \<open>\<v>\<a>\<l> 10 \<Ztypecolon> \<nat>\<close>
-  is [routine]
+  is [routine]   
   \<medium_left_bracket> $x \<rightarrow> var v (*x is an immutable value, and here we assign it to a variable v*);;
     while \<open>x \<Ztypecolon> ?T \<s>\<u>\<b>\<j> x. Inv: (x \<le> 10) \<and> Guard: True \<and> End: (x = 10)\<close> (*annotation*)
     \<medium_left_bracket> \<open>True\<close> \<medium_right_bracket>. (*guard*)
     \<medium_left_bracket>
-      if \<open>$v = 10\<close> \<medium_left_bracket> break \<medium_right_bracket>. \<medium_left_bracket> \<open>$v + 1\<close> \<rightarrow> v;; continue \<medium_right_bracket>.
+      if ;; \<open>$v = 10\<close> \<medium_left_bracket> break \<medium_right_bracket>. \<medium_left_bracket> \<open>$v + 1\<close> \<rightarrow> v;; continue \<medium_right_bracket>.
       assert \<bottom>
     \<medium_right_bracket>. (*loop body*)
     $v
